\subsubsection{Full Load}
Both the primary and secondary switches are turned on resulting in a full load on the circuit.
\begin{figure}[H]
	\centering
	
	\begin{circuitikz} [american voltages] \draw
    
    (0,0) to[vsourcesin, l=$V_{2}$] node[label=\textcircled{1}] {} (0,5)
    (0,5) to[battery1, l=$2V_{th}$] (1.9,5)
    (1.5,5) to[R,l=$2R_b$,i=$i_d$, v=$V_d$] (4.5,5)
    (4.5,5) to[nos,o-o] (6,5)
    
    (6,5) node[label=\textcircled{2}] {} to[capacitor, i=$i_c$, l=$C$,v=$V_c$] (6,0)
    
    (6,5) to[R,l=$R_s$,i=$i_s$] (9,5)
    
    (9,5) node[label=\textcircled{3}] {} to[battery1, l=$V_z$] (9,4)
    (9,4) to[R, l=$R_z$, i=$i_z$] (9,2)
    (9,2) to[nos,o-o] (9,0.5)
    (9,0.5) to[short] (9,0)
    
    (12,5) node[label=\textcircled{4}] {} to[R,l=$R_{L_1}$,i=$i_{l_1}$] (12,0)
    (12,5) to[short] (15,5)
    (15,5) node[label=\textcircled{5}] {} to[R,l=$R_{L_2}$,i=$i_{l_2}$] (15,3)
    (15,3) to[inductor,l=$L$,i=$i_l$] (15,0)
    
    (9,5) to[short,i=$i_{l_{12}}$] (12,5)
    (0,0) to[short] (15,0)
    (7.5,0) node[ground]{} (5,-1);
    
    \end{circuitikz}
	
	\label{circ:full_load}
	\caption{Power supply circuit with the full load applied}
\end{figure}

\paragraph{Nodal Analysis}
\subparagraph{Node \textcircled{2}}
Determine an expression for $i_d(t)$ at node \textcircled{2} using KCL
\begin{equation}
	\begin{split}
		i_d(t) &= i_c(t) + i_s \\
		\sbracket{\frac{\frac{e_1 - e_2}{2} - V_{th}}{R_b}}\cdot u\bracket{\frac{e_1 - e_2}{2} - V_{th}} &= C \frac{d(e_2)}{dt} + \frac{e_2 - e_3}{R_s}
	\end{split}
	\label{eq:fullLoad_node2}
\end{equation}

\subparagraph{Node \textcircled{3}}
Determine an expression for $i_s$ at node \textcircled{3} using KCL
\begin{equation}
	\begin{split}
		i_s &= i_z + i_{l} \\
		\frac{e_2 - e_3}{R_s} &= \frac{e_3 - V_z}{R_z} + i_{l_{12}}
	\end{split}
	\label{eq:fullLoad_node3}
\end{equation}

\subparagraph{Node \textcircled{4}}
Determine an expression for $i_{l_{12}}$ at node \textcircled{4} using KCL
\begin{equation}
	\begin{split}
		i_{l_{12}} &= i_{l_1} + i_{l_2} \\
		    &= \frac{e_4}{R_{L_1}} + \frac{e_4 - e_5}{R_{L_2}}
	\end{split}
\end{equation}
Note $e_4 = e_3$ and $e_4 = e_5$ as there are no voltage drops across these terminals.
\begin{equation}
	\begin{split}
	 \therefore i_{l_{12}} = \frac{e_3}{R_{L_1}} + \frac{e_3 - e_4}{R_{L_2}}
	\end{split}
	\label{eq:fullLoad_node4}
\end{equation}
Recalling the ideal inductor model in \eqref{eq:ideal_inductor} the rate of change of $i_{l}$ related to output voltage $e_4$ by,
\begin{equation}
	\begin{split}
		e_4 = L\frac{di_l}{dt} = L\frac{di_{l_2}}{dt}
	\end{split}
	\label{eq:fullLoad_output}
\end{equation}

\paragraph{Differential Equations}
The current $i_s$ depends on the biasing of the zener diode. The biasing of the zener is determined by the relation between $e_3$ and $V_z$. Two set of differential equations are derived based on the operation of the Zener.

\subparagraph{Reverse Bias}
When $e_3 < V_z$ the zener is in reverse bias. There is no additional current flow at node \textcircled{3} as the switch remains open. Thus, the current flowing into node \textcircled{3} $i_s$ is just given by $$i_s = i_{l_{12}} = i_{l_1} + i_{l_2}$$
Note: Current $i_{l_2}$ equals $i_l$
\begin{equation}
	\frac{e_2 - e_3}{R_s} = \frac{e_3}{R_{L_1}} + i_l
	\label{eq:node3}
\end{equation}
In this state, the system is characterised by these set of equations
\begin{align}
	i_c(t) + i_s &= \sbracket{\frac{\frac{e_1 - e_2}{2} - V_{th}}{R_b}}\cdot u\bracket{\frac{e_1 - e_2}{2} - V_{th}} \\
	i_s &= \frac{e_3}{R_{L_1}} + i_l \\
	i_c(t) &= C \frac{de_2}{d_t} \\
	e_4 &= L\frac{di_l}{dt} = e_3 - R_{L_2}i_l
	\label{eq:fullLoad_system}
\end{align}
Solving \eqref{eq:node3} for $e_3$ gives an expression for the voltage at node \textcircled{3}
\begin{equation}
\begin{split}
	e_3 &= \frac{e_2R_{L_1} - i_l R_s R_{L_1}}{R_s + R_{L_1}} \\
	    &= \bracket{\frac{e_2 - R_s i_l}{R_{L_1} + R_s}}R_{L_1}
\end{split}
\label{eq:e3_il}
\end{equation}
Substitute $e_3$ into the expression for $i_s$ from \eqref{eq:fullLoad_system}
\begin{equation}
 \begin{split}
	i_s &= \frac{\bracket{\frac{e_2 - R_s i_l}{R_{L_1} + R_s}}R_{L_1}}{R_{L_1}} + i_l \\
		&= \frac{e_2 - R_s i_l}{R_{L_1} + R_s} + i_l
 \end{split}
\end{equation}
Hence, the current across the capacitor $i_c(t)$ is:
\begin{equation}
	i_c(t) = \sbracket{\frac{\frac{e_1 - e_2}{2} - V_{th}}{R_b}}\cdot u\bracket{\frac{e_1 - e_2}{2} - V_{th}} - \frac{e_2 - R_s i_l}{R_{L_1} + R_s} - i_l
\end{equation}
and it's resulting differential equation is,
\begin{equation}
	\frac{de_2}{dt} = \frac{1}{c}\bracket{\sbracket{\frac{\frac{e_1 - e_2}{2} - V_{th}}{R_b}}\cdot u\bracket{\frac{e_1 - e_2}{2} - V_{th}} - \frac{e_2 - R_s i_l}{R_{L_1} + R_s} - i_l}
	\label{eq:fullLoad_DiffEq1}
\end{equation}
This condition only holds true when $e_3 < V_z$.

\pagebreak
Another differential equation can be found relating the rate of change of $i_l$ to the inductance from the system of equations in \eqref{eq:fullLoad_system}.
\begin{equation}
	\begin{split}
		L\frac{di_l}{dt} &= \bracket{\frac{e_2 - R_s i_l}{R_{L_1} + R_s}}R_{L_1} - R_{L_2}i_l \\
		 \frac{di_l}{dt} &= \frac{1}{L} \sbracket{
		 	\bracket{\frac{e_2 - R_s i_l}{R_{L_1} + R_s}}R_{L_1} - R_{L_2}i_l
		 }
	\end{split}
	\label{eq:fullLoad_DiffEq2}
\end{equation}
This also only holds true when $e_3 < V_z$, or, when
\begin{equation}
	\bracket{\frac{e_2 - R_s i_l}{R_{L_1} + R_s}}R_{L_1} < V_z
\end{equation}

\subparagraph{Forward Bias}
When $e_3 \geq V_z$ the zener is in reverse bias. The current flow in node \textcircled{3} must be accounted for as the switch remains closed. Thus, the current flowing into node \textcircled{3} $i_s$ is just given by $$i_s = i_{l_{12}} + i_z = i_{l_1} + i_l + i_z$$
\begin{equation}
	\frac{e_2 - e_3}{R_s} = \frac{e_3}{R_{L_1}} + \frac{e_3 - V_z}{R_z} + i_l
	\label{eq:forwardBias_node3}
\end{equation}
In this state, the system is characterised by these set of equations
\begin{align}
	i_c(t) + i_s &= \sbracket{\frac{\frac{e_1 - e_2}{2} - V_{th}}{R_b}}\cdot u\bracket{\frac{e_1 - e_2}{2} - V_{th}} \\
	i_s &= \frac{e_3}{R_{L_1}} + \frac{e_3 - V_z}{R_z} + i_l \\
	i_c(t) &= C \frac{de_2}{d_t} \\
	e_4 &= L\frac{di_l}{dt} = e_3 - R_{L_2}i_l
	\label{eq:fullLoad_forwardBias_system}
\end{align}
Solving \eqref{eq:forwardBias_node3} for $e_3$ gives an expression for the voltage at node \textcircled{3}
\begin{equation}
\begin{split}
	e_3\left(\frac{1}{R_{L_1}} + \frac{1}{R_z} + \frac{1}{R_s}\right) = \frac{e_2}{R_s} + \frac{V_z}{R_z} + i_l \\
		e_3 = \frac{\frac{e_2}{R_s} + \frac{V_z}{R_z} + i_l}{\frac{1}{R_{L_1}} + \frac{1}{R_z} + \frac{1}{R_s}}
\end{split}
\label{eq:fullLoad_forwardBias_e3_unsimplified}
\end{equation}
Multiply the numerator and denominator of \eqref{eq:fullLoad_forwardBias_e3_unsimplified} by  $R_sR_zR_{L_1}$
\begin{equation}
 e_3 = \frac{e_2 R_z R_{L_1} + V_z R_s R_{L_1} + i_l R_s R_z}{R_z R_{L_1} + R_s R_{L_1} + R_s R_z}
\label{eq:fullLoad_forwardBias_e3}
\end{equation}
Substitute $e_3$ into the expression for $i_s$ from \eqref{eq:fullLoad_forwardBias_system},
\begin{equation}
i_s = \frac{e_2}{R_s} \left(\frac{R_z R_{L_1}}{R_s R_{L_1} + R_z R_{L_1} + R_s R_z}\right) + \frac{V_z R_{L_1}}{R_s R_{L_1} + R_z R_{L_1} + R_s R_z} - \frac{i_l R_s}{R_s R_{L_1} + R_z R_{L_1} + R_s R_z} + i_l
\end{equation}
Then, simplify the above expression:
\begin{equation}
i_s = \frac{e_2 (R_z + R_{L_1}) - V_z R_{L_1} + i_l R_z R_{L_1}}{R_z R_s + R_{L_1} R_z + R_s R_{L_1}}
\end{equation}
Hence, the current across the capacitor $i_c(t)$ is:
\begin{equation}
	i_c(t) = \sbracket{\frac{\frac{e_1 - e_2}{2} - V_{th}}{R_b}}\cdot u\bracket{\frac{e_1 - e_2}{2} - V_{th}} - \frac{e_2 (R_z + R_{L_1}) - V_z R_{L_1} + i_l R_z R_{L_1}}{R_z R_s + R_{L_1} R_z + R_s R_{L_1}}
\end{equation}
and it's resulting differential equation is,
\begin{equation}
	\frac{de_2}{dt} = \frac{1}{C}\bracket{\sbracket{\frac{\frac{e_1 - e_2}{2} - V_{th}}{R_b}}\cdot u\bracket{\frac{e_1 - e_2}{2} - V_{th}} - \frac{e_2 (R_z + R_{L_1}) - V_z R_{L_1} + i_l R_z R_{L_1}}{R_z R_s + R_{L_1} R_z + R_s R_{L_1}}}
	\label{eq:fullLoad_DiffEq3}
\end{equation}
This condition only holds true when $e_3 \geq V_z$. Another differential equation can be found relating the rate of change of $i_l$ to the inductance from the system of equations in \eqref{eq:fullLoad_forwardBias_system}.
\begin{equation}
	\begin{split}
		L\frac{di_l}{dt} &= \frac{e_2 R_z R_{L_1} + V_z R_s R_{L_1} + i_l R_s R_z}{R_z R_{L_1} + R_s R_{L_1} + R_s R_z} - R_{L_2}i_l \\
		 \frac{di_l}{dt} &= \frac{1}{L} \sbracket{\frac{e_2 R_z R_{L_1} + V_z R_s R_{L_1} + i_l R_s R_z}{R_z R_{L_1} + R_s R_{L_1} + R_s R_z} - R_{L_2}i_l}
	\end{split}
	\label{eq:fullLoad_DiffEq4}
\end{equation}
This also only holds true when $e_3 \geq V_z$, or, when
\begin{equation}
	\bracket{\frac{e_2 - R_s i_l}{R_{L_1} + R_s}}R_{L_1} \geq V_z
\end{equation}

Thus, four differential equations \eqref{eq:fullLoad_DiffEq1}, \eqref{eq:fullLoad_DiffEq2}, \eqref{eq:fullLoad_DiffEq3}, \eqref{eq:fullLoad_DiffEq4} have been derived characterising the operation of the circuit under full load conditions.

